clean up BitBlat/BoolExpr

LeanSAT/BitBlast/BoolExpr/Basic.lean
@@ -3,11 +3,7 @@ Copyright (c) 2024 Lean FRO, LLC. All rights reserved.
 Released under Apache 2.0 license as described in the file LICENSE.
 Authors: Scott Morrison
 -/
-import LeanSAT.Sat
-
 set_option linter.missingDocs false
-
-open Lean Meta Sat
 
 inductive Gate
 | and
@@ -59,25 +55,25 @@ def size : BoolExpr α → Nat
 theorem size_pos (x : BoolExpr α) : 0 < x.size := by
   cases x <;> simp [size] <;> omega
 
-def eval (f : α → Bool) : BoolExpr α → Bool
-  | .literal a => f a
+def eval (a : α → Bool) : BoolExpr α → Bool
+  | .literal l => a l
   | .const b => b
-  | .not x => !eval f x
-  | .gate g x y => g.eval (eval f x) (eval f y)
+  | .not x => !eval a x
+  | .gate g x y => g.eval (eval a x) (eval a y)
 
-@[simp] theorem eval_literal : eval f (.literal a) = f a := rfl
-@[simp] theorem eval_const : eval f (.const b) = b := rfl
-@[simp] theorem eval_not : eval f (.not x) = !eval f x := rfl
-@[simp] theorem eval_gate : eval f (.gate g x y) = g.eval (eval f x) (eval f y) := rfl
+@[simp] theorem eval_literal : eval a (.literal l) = a l := rfl
+@[simp] theorem eval_const : eval a (.const b) = b := rfl
+@[simp] theorem eval_not : eval a (.not x) = !eval a x := rfl
+@[simp] theorem eval_gate : eval a (.gate g x y) = g.eval (eval a x) (eval a y) := rfl
 
-def sat (f : α → Bool) (x : BoolExpr α) : Prop := eval f x = true
+def Sat (a : α → Bool) (x : BoolExpr α) : Prop := eval a x = true
 def Unsat (x : BoolExpr α) : Prop := ∀ f, eval f x = false
 
-theorem sat_and {x y : BoolExpr α} {f : α → Bool} (hx : sat f x) (hy : sat f y)
-    : sat f (BoolExpr.gate .and x y) := by
-  simp only [sat] at *
+theorem sat_and {x y : BoolExpr α} {a : α → Bool} (hx : Sat a x) (hy : Sat a y) :
+    Sat a (BoolExpr.gate .and x y) := by
+  simp only [Sat] at *
   simp [hx, hy, Gate.eval]
 
-theorem sat_true {f : α → Bool} : sat f (BoolExpr.const true : BoolExpr α) := rfl
+theorem sat_true {a : α → Bool} : Sat a (BoolExpr.const true : BoolExpr α) := rfl
 
 end BoolExpr
