LeanSAT/BitBlast/BoolExpr/BitBlast.lean
@@ -21,17 +21,16 @@ open Std.Sat
 
 variable {β : Type} [Hashable β] [DecidableEq β]
 
-
 /--
-Turn a `BoolExpr` into an AIG + entrypoint.
+Turn a `BoolExpr` into an `Entrypoint`.
 -/
 def ofBoolExprCached (expr : BoolExpr α) (atomHandler : AIG β → α → Entrypoint β)
     [LawfulOperator β (fun _ => α) atomHandler] : Entrypoint β :=
   go expr AIG.empty atomHandler |>.val
 where
   go (expr : BoolExpr α) (aig : AIG β) (atomHandler : AIG β → α → Entrypoint β)
-      [LawfulOperator β (fun _ => α) atomHandler]
-      : ExtendingEntrypoint aig :=
+      [LawfulOperator β (fun _ => α) atomHandler] :
+      ExtendingEntrypoint aig :=
     match expr with
     | .literal var => ⟨atomHandler aig var, by apply LawfulOperator.le_size⟩
     | .const val => ⟨aig.mkConstCached val, (by apply LawfulOperator.le_size)⟩
@@ -51,31 +50,30 @@ where
       | .and =>
         let ret := aig.mkAndCached input
         have := LawfulOperator.le_size (f := mkAndCached) aig input
-        -- TODO: why two dsimp calls???????
-        ⟨ret, by dsimp [ret] at *; dsimp at rextend; omega⟩
+        ⟨ret, by dsimp only [ret] at lextend rextend ⊢; omega⟩
       | .or =>
         let ret := aig.mkOrCached input
         have := LawfulOperator.le_size (f := mkOrCached) aig input
-        ⟨ret, by dsimp [ret] at *; dsimp at rextend; omega⟩
+        ⟨ret, by dsimp only [ret] at lextend rextend ⊢; omega⟩
       | .xor =>
         let ret := aig.mkXorCached input
         have := LawfulOperator.le_size (f := mkXorCached) aig input
-        ⟨ret, by dsimp [ret] at *; dsimp at rextend; omega⟩
+        ⟨ret, by dsimp only [ret] at lextend rextend ⊢; omega⟩
       | .beq =>
         let ret := aig.mkBEqCached input
         have := LawfulOperator.le_size (f := mkBEqCached) aig input
-        ⟨ret, by dsimp [ret] at *; dsimp at rextend; omega⟩
+        ⟨ret, by dsimp only [ret] at lextend rextend ⊢; omega⟩
       | .imp =>
         let ret := aig.mkImpCached input
         have := LawfulOperator.le_size (f := mkImpCached) aig input
-        ⟨ret, by dsimp [ret] at *; dsimp at rextend; omega⟩
+        ⟨ret, by dsimp only [ret] at lextend rextend ⊢; omega⟩
 
 
 variable (atomHandler : AIG β → α → Entrypoint β) [LawfulOperator β (fun _ => α) atomHandler]
 
 theorem ofBoolExprCached.go_decls_size_le (expr : BoolExpr α) (aig : AIG β) :
-    aig.decls.size ≤ (ofBoolExprCached.go expr aig atomHandler).val.aig.decls.size := by
-  exact (ofBoolExprCached.go expr aig atomHandler).property
+    aig.decls.size ≤ (ofBoolExprCached.go expr aig atomHandler).val.aig.decls.size :=
+  (ofBoolExprCached.go expr aig atomHandler).property
 
 theorem ofBoolExprCached.go_decl_eq (idx) (aig : AIG β) (h : idx < aig.decls.size) (hbounds) :
     (ofBoolExprCached.go expr aig atomHandler).val.aig.decls[idx]'hbounds = aig.decls[idx] := by
@@ -100,27 +98,22 @@ theorem ofBoolExprCached.go_decl_eq (idx) (aig : AIG β) (h : idx < aig.decls.si
     cases g with
     | and =>
       simp only [go]
-      rw [AIG.LawfulOperator.decl_eq (f := mkAndCached)]
-      rw [rih, lih]
+      rw [AIG.LawfulOperator.decl_eq (f := mkAndCached), rih, lih]
     | or =>
       simp only [go]
-      rw [AIG.LawfulOperator.decl_eq (f := mkOrCached)]
-      rw [rih, lih]
+      rw [AIG.LawfulOperator.decl_eq (f := mkOrCached), rih, lih]
     | xor =>
       simp only [go]
-      rw [AIG.LawfulOperator.decl_eq (f := mkXorCached)]
-      rw [rih, lih]
+      rw [AIG.LawfulOperator.decl_eq (f := mkXorCached), rih, lih]
     | beq =>
       simp only [go]
-      rw [AIG.LawfulOperator.decl_eq (f := mkBEqCached)]
-      rw [rih, lih]
+      rw [AIG.LawfulOperator.decl_eq (f := mkBEqCached), rih, lih]
     | imp =>
       simp only [go]
-      rw [AIG.LawfulOperator.decl_eq (f := mkImpCached)]
-      rw [rih, lih]
+      rw [AIG.LawfulOperator.decl_eq (f := mkImpCached), rih, lih]
 
-theorem ofBoolExprCached.go_IsPrefix_aig {aig : AIG β}
-    : IsPrefix aig.decls (go expr aig atomHandler).val.aig.decls := by
+theorem ofBoolExprCached.go_IsPrefix_aig {aig : AIG β} :
+    IsPrefix aig.decls (go expr aig atomHandler).val.aig.decls := by
   apply IsPrefix.of
   . intro idx h
     apply ofBoolExprCached.go_decl_eq
@@ -128,7 +121,7 @@ theorem ofBoolExprCached.go_IsPrefix_aig {aig : AIG β}
 
 
 @[simp]
-theorem ofBoolExprCached.go_denote_entry (entry : Entrypoint β) {h}:
+theorem ofBoolExprCached.go_denote_entry (entry : Entrypoint β) {h} :
     ⟦(go expr entry.aig atomHandler).val.aig, ⟨entry.ref.gate, h⟩, assign ⟧
       =
     ⟦entry, assign⟧ := by
@@ -153,8 +146,8 @@ theorem ofBoolExprCachedDirect_eval_eq_eval (expr : BoolExpr α) (assign) :
     ⟦ofBoolExprCachedDirect expr, assign⟧ = expr.eval assign := by
   apply ofBoolExprCached.go_eval_eq_eval
 
-theorem ofBoolExprCachedDirect_unsat_iff {expr : BoolExpr α}
-    : (ofBoolExprCachedDirect expr).Unsat ↔ expr.Unsat := by
+theorem ofBoolExprCachedDirect_unsat_iff {expr : BoolExpr α} :
+    (ofBoolExprCachedDirect expr).Unsat ↔ expr.Unsat := by
   constructor
   all_goals
     intro h assign
